Proofs

compiler/backend/flat_scopeAnalysisScript.sml
@@ -1,244 +1,203 @@
 open
   preamble
   flatLangTheory
-  mlintTheory
+  mlnumTheory
 
 (* Used to give all identifiers a unique name *)
 val _ = new_theory "flat_scopeAnalysis";
 
-val mk_unique_name_def = Define`
-  mk_unique_name n s =
-    CONCAT [explode (mlint$toString n); "_"; s]
-`
+val mk_unique_name_def = Define
 
-val compile_p_def = tDefine "compile_p" `
-  ( compile_p counter repl Pany =
-      (counter, repl, Pany)
-  ) ∧ (
+  `mk_unique_name n s = CONCAT [explode (mlnum$toString n); "_"; s]`
+
+val compile_p_def = tDefine "compile_p"
+
+  `(compile_p counter repl Pany = (counter, repl, Pany)) ∧ (
     compile_p counter repl (Pvar x) =
       let newName = mk_unique_name counter x in
-      (counter + 1, (x, newName)::repl, Pvar newName)
-  ) ∧ (
-    compile_p counter repl (Plit lit) =
-      (counter, repl, Plit lit)
-  ) ∧ (
+      (counter + 1, (x, newName)::repl, Pvar newName)) ∧ (
+    compile_p counter repl (Plit lit) = (counter, repl, Plit lit)) ∧ (
     compile_p counter repl (Pcon id l) =
       let (counter, repl, l) = compile_ps counter repl l in
-      (counter, repl, Pcon id l)
-  ) ∧ (
+      (counter, repl, Pcon id l)) ∧ (
     compile_p counter repl (Pref p) =
       let (counter, repl, p) = compile_p counter repl p in
-      (counter, repl, Pref p)
-  ) ∧ (
-    compile_ps counter repl [] =
-      (counter, repl, [])
-  ) ∧ (
+      (counter, repl, Pref p)) ∧ (
+    compile_ps counter repl [] = (counter, repl, [])) ∧ (
     compile_ps counter repl (p::ps) =
       let (counter, repl, p) = compile_p counter repl p in
       let (counter, repl, ps) = compile_ps counter repl ps in
-      (counter, repl, p::ps)
-  )
-`
-( WF_REL_TAC `inv_image $< (λ x. (case x of
+      (counter, repl, p::ps))`
+
+  (WF_REL_TAC `inv_image $< (λ x. (case x of
   | INL (_, _, p) => pat_size p
   | INR (_, _, ps) => pat1_size ps
-  ))`
-)
+  ))`)
 
-val compile_name_rec_fun_def = Define`
-  compile_name_rec_fun counter repl (fName, vName, e) =
-    let newFName = mk_unique_name counter fName in
-    counter + 1,
-    (fName, newFName)::repl,
-    (newFName, vName, e)
-`
+val compile_name_rec_funs_def = Define
 
-val compile_name_rec_funs_def = Define`
-  ( compile_name_rec_funs counter repl [] =
-      (counter, repl, [])
-  ) ∧ (
-    compile_name_rec_funs counter repl (f::funs) =
-      let (counter, repl, f) = compile_name_rec_fun counter repl f in
-      let (counter, repl, funs) = compile_name_rec_funs counter repl funs in
-      (counter, repl, f::funs)
-  )
-`
+  `(compile_name_rec_funs counter repl [] = (counter, repl, [])) ∧ (
+    compile_name_rec_funs counter repl ((fName, vName, e)::funs) =
+      let newFName = mk_unique_name counter fName in
+      let (counter, repl, funs) = compile_name_rec_funs (counter + 1) repl funs in
+      (counter, (fName, newFName)::repl, (newFName, vName, e)::funs))`
 
-val compile_name_rec_funs_LENGTH = Q.store_thm(
-  "compile_name_rec_funs_LENGTH",
-  `∀ counter repl funs counter' repl' funs'.
-     (counter',repl',funs') = compile_name_rec_funs counter repl funs
-     ⇒ LENGTH funs' = LENGTH funs`,
-  Induct_on`funs` >>
-  rw[compile_name_rec_funs_def,compile_name_rec_fun_def,exp_size_def] >>
-  Cases_on`h` >> Cases_on`r` >>
-  fs[mk_unique_name_def,exp_size_def,compile_name_rec_fun_def] >>
-  qmatch_asmsub_abbrev_tac`compile_name_rec_funs counter0 repl0 _` >>
-  Cases_on`(compile_name_rec_funs counter0 repl0 funs)` >>
-  Cases_on`r` >>
-  first_x_assum (assume_tac o Q.SPECL[`counter0`,`repl0`]) >>
-  rfs[]);
+val p_size_bis = Define
 
-val compile_exp_def = tDefine "compile_exp" `
-  ( compile_exp counter repl (Raise t e) =
-      let (counter, e) = compile_exp counter repl e in
-      (counter, Raise t e)
-  ) ∧ (
+  `(p_size_bis Pany : num      = 1                                 ) ∧ (
+    p_size_bis (Pvar _)   = 1                                 ) ∧ (
+    p_size_bis (Plit _)   = 1                                 ) ∧ (
+    p_size_bis (Pcon _ l) = 1 + ps_size_bis l                 ) ∧ (
+    p_size_bis (Pref p)   = 1 + p_size_bis p                  ) ∧ (
+    ps_size_bis []        = 1                                 ) ∧ (
+    ps_size_bis (h::t)    = 1 + p_size_bis h + ps_size_bis t  )`
+
+val exp_size_bis_def = tDefine "exp_size_bis"
+
+  `(exp_size_bis (Raise _ e)        = 1 + exp_size_bis e                                      ) ∧ (
+    exp_size_bis (Handle _ e pes)   = 1 + exp_size_bis e + pes_size_bis pes                   ) ∧ (
+    exp_size_bis (Lit _ _)          = 1                                                       ) ∧ (
+    exp_size_bis (Con _ _ es)       = 1 + exps_size_bis es                                    ) ∧ (
+    exp_size_bis (Var_local _ _)    = 1                                                       ) ∧ (
+    exp_size_bis (Fun _ _ e)        = 1 + exp_size_bis e                                      ) ∧ (
+    exp_size_bis (App _ _ es)       = 1 + exps_size_bis es                                    ) ∧ (
+    exp_size_bis (If _ e1 e2 e3)    = 1 + exp_size_bis e1 + exp_size_bis e2 + exp_size_bis e3 ) ∧ (
+    exp_size_bis (Mat _ e pes)      = 1 + exp_size_bis e + pes_size_bis pes                   ) ∧ (
+    exp_size_bis (Let _ _ e1 e2)    = 1 + exp_size_bis e1 + exp_size_bis e2                   ) ∧ (
+    exp_size_bis (Letrec _ funs e)  = 1 + funs_size_bis funs + exp_size_bis e                 ) ∧ (
+    fun_size_bis (_, e)             = 1 + exp_size_bis e                                      ) ∧ (
+    funs_size_bis []                = 1                                                       ) ∧ (
+    funs_size_bis ((_, f)::t)       = 1 + fun_size_bis f + funs_size_bis t                    ) ∧ (
+    exps_size_bis []                = 1                                                       ) ∧ (
+    exps_size_bis (e::es)           = 1 + exp_size_bis e + exps_size_bis es                   ) ∧ (
+    pe_size_bis (p, e)              = 1 + p_size_bis p + exp_size_bis e                       ) ∧ (
+    pes_size_bis []                 = 1                                                       ) ∧ (
+    pes_size_bis (pe::t)            = 1 + pe_size_bis pe + pes_size_bis t                     )`
+
+  ( WF_REL_TAC `inv_image $< ( λ x . ( case x of
+  | INL e => exp_size e
+  | INR (INL f) => exp4_size f
+  | INR (INR (INL funs)) => exp1_size funs
+  | INR (INR (INR (INL es))) => exp6_size es
+  | INR (INR (INR (INR (INL pe)))) => exp5_size pe
+  | INR (INR (INR (INR (INR pes)))) => exp3_size pes))`)
+
+val compile_nrf_size = Q.store_thm("compile_nrf_size",
+
+  `∀ l c r. funs_size_bis l = funs_size_bis (SND (SND (compile_name_rec_funs c r l)))`,
+
+   Induct
+>> rw[compile_name_rec_funs_def]
+>> Cases_on `h`
+>> Cases_on `r'`
+>> fs[compile_name_rec_funs_def]
+>> pairarg_tac
+>> fs[]
+>> metis_tac[exp_size_bis_def, SND])
+
+val compile_exp_def = tDefine "compile_exp"
+`(compile_exp counter repl (Raise t e) =
+      let (counter, e) = compile_exp counter repl e in (counter, Raise t e)) ∧ (
     compile_exp counter repl (Handle t e pes) =
       let (counter, e) = compile_exp counter repl e in
       let (counter, pes) = compile_pes counter repl pes in
-      (counter, Handle t e pes)
-  ) ∧ (
-    compile_exp counter repl (Lit t l) =
-      (counter, Lit t l)
-  ) ∧ (
+      (counter, Handle t e pes)) ∧ (
+    compile_exp counter repl (Lit t l) = (counter, Lit t l)) ∧ (
     compile_exp counter repl (Con t id es) =
       let (counter, es) = compile_exps counter repl es in
-      (counter, Con t id es)
-  ) ∧ (
+      (counter, Con t id es)) ∧ (
     compile_exp counter repl (Var_local t x) =
       (* TODO: in the case of NONE, we should rename x (and add (x, newX) to the
       * repl ? maybe not...), this will avoid crash when something is undefined, it will not
       * append after passng through the stdlib and typechecking, but when
       * debugging, if we use something like equality test or addition, then
         * it'll not work... *)
-      (counter, Var_local t (case ALOOKUP repl x of | NONE => x | SOME x => x))
-  ) ∧ (
+      (counter, Var_local t (case ALOOKUP repl x of | NONE => x | SOME x => x))) ∧ (
     compile_exp counter repl (Fun t x e) =
       let newName = mk_unique_name counter x in
       let (counter, e) = compile_exp (counter + 1) ((x, newName)::repl) e in
-      (counter, Fun t newName e)
-  ) ∧ (
+      (counter, Fun t newName e)) ∧ (
     compile_exp counter repl (App t op es) =
       let (counter, es) = compile_exps counter repl es in
-      (counter, App t op es)
-  ) ∧ (
+      (counter, App t op es)) ∧ (
     compile_exp counter repl (If t e1 e2 e3) =
       let (counter, e1) = compile_exp counter repl e1 in
       let (counter, e2) = compile_exp counter repl e2 in
       let (counter, e3) = compile_exp counter repl e3 in
-      (counter, If t e1 e2 e3)
-  ) ∧ (
+      (counter, If t e1 e2 e3)) ∧ (
     compile_exp counter repl (Mat t e pes) =
       let (counter, e) = compile_exp counter repl e in
       let (counter, pes) = compile_pes counter repl pes in
-      (counter, Mat t e pes)
-  ) ∧ (
+      (counter, Mat t e pes)) ∧ (
     compile_exp counter repl (Let t (SOME x) e1 e2) =
       let newName = mk_unique_name counter x in
       let (counter, e1) = compile_exp (counter + 1) repl e1 in
       let (counter, e2) = compile_exp counter ((x, newName)::repl) e2 in
-      (counter, Let t (SOME newName) e1 e2)
-  ) ∧ (
+      (counter, Let t (SOME newName) e1 e2)) ∧ (
     compile_exp counter repl (Let t NONE e1 e2) =
       let (counter, e1) = compile_exp counter repl e1 in
       let (counter, e2) = compile_exp counter repl e2 in
-      (counter, Let t NONE e1 e2)
-  ) ∧ (
+      (counter, Let t NONE e1 e2)) ∧ (
     compile_exp counter repl (Letrec t funs e) =
       let (counter, repl, funs) = compile_name_rec_funs counter repl funs in
       let (counter, funs) = compile_funs counter repl funs in
       let (counter, e) = compile_exp counter repl e in
-      (counter, Letrec t funs e)
-  ) ∧ (
+      (counter, Letrec t funs e)) ∧ (
     compile_fun counter repl (vName, e) =
       let newVName = mk_unique_name counter vName in
       let (counter, e) = compile_exp (counter + 1) ((vName, newVName)::repl) e in
-      (counter, (newVName, e))
-  ) ∧ (
-    compile_funs counter repl [] =
-      (counter, [])
-  ) ∧ (
+      (counter, (newVName, e))) ∧ (
+    compile_funs counter repl [] = (counter, [])) ∧ (
     compile_funs counter repl ((fName, f)::funs) =
       let (counter, f) = compile_fun counter repl f in
       let (counter, funs) = compile_funs counter repl funs in
-      (counter, (fName, f)::funs)
-  ) ∧ (
-    compile_exps counter repl [] =
-      (counter, [])
-  ) ∧ (
+      (counter, (fName, f)::funs)) ∧ (
+    compile_exps counter repl [] = (counter, [])) ∧ (
     compile_exps counter repl (e::es) =
       let (counter, e) = compile_exp counter repl e in
       let (counter, es) = compile_exps counter repl es in
-      (counter, e::es)
-  ) ∧ (
+      (counter, e::es)) ∧ (
     compile_pe counter repl pe =
       let (p, e) = pe in
       let (counter, repl, p) = compile_p counter repl p in
       let (counter, e) = compile_exp counter repl e in
-      (counter, (p, e))
-  ) ∧ (
-    compile_pes counter repl [] =
-      (counter, [])
-  ) ∧ (
+      (counter, (p, e))) ∧ (
+    compile_pes counter repl [] = (counter, [])) ∧ (
     compile_pes counter repl (pe::pes) =
       let (counter, pe) = compile_pe counter repl pe in
       let (counter, pes) = compile_pes counter repl pes in
-      (counter, pe::pes)
-  )`
-  cheat
-(* This will not work, to do it correctly we've got to write a another exp_size function which doesn't use the var/fun name length ...
-(
- WF_REL_TAC `inv_image $< ( λ x . ( case x of
-    | INL (counter, repl, e) => exp_size e
-    | INR (INL (counter, repl, f)) => exp4_size f
-    | INR (INR (INL (counter, repl, funs))) => exp1_size funs
-    | INR (INR (INR (INL (counter, repl, es)))) => exp6_size es
-    | INR (INR (INR (INR (INL (counter, repl, pe))))) => exp5_size pe
-    | INR (INR (INR (INR (INR (counter, repl, pes))))) => exp3_size pes
-  ))` >>
-  simp[exp_size_def] >>
-  rw[]
-      imp_res_tac compile_name_rec_funs_LENGTH >>
-      last_x_assum (fn hyp => assume_tac (GSYM hyp)) >>
-      fs[]
-      ) >>
+      (counter, pe::pes))`
 
+   ( WF_REL_TAC `inv_image $< (λ x. (case x of
+   | INL (counter, repl, e) => exp_size_bis e
+   | INR (INL (counter, repl, f)) => fun_size_bis f
+   | INR (INR (INL (counter, repl, funs))) => funs_size_bis funs
+   | INR (INR (INR (INL (counter, repl, es)))) => exps_size_bis es
+   | INR (INR (INR (INR (INL (counter, repl, pe))))) => pe_size_bis pe
+   | INR (INR (INR (INR (INR (counter, repl, pes))))) => pes_size_bis pes))`
 
-  CASE_TAC >> fs[]
-  CASE_TAC >> fs[]
+>> rw[exp_size_bis_def]
+>> CASE_TAC
+>> CASE_TAC
+>> rw[]
+>> `funs_size_bis funs' = funs_size_bis funs` by metis_tac[compile_nrf_size, SND]
+>> rw[])
 
-  >> Induct_on `funs`
-  >> simp [compile_name_rec_funs_def]
-  >> simp [compile_name_rec_fun_def]
-  >> rw[]
+val compile_dec_def = Define
 
-  >> Induct_on `funs`
-  >> Induct_on `funs'`
-  >> simp[mk_unique_name_def]
-  >> rfs[]
-  >> Cases_on `h`
-  >> Cases_on `r`
-  >> res_tac
-  >> Cases_on `e`
-  >> metis_tac[]
-  >> cheat
-)
-*)
+  `(compile_dec counter (Dlet e) = let (counter, e) = compile_exp counter [] e in (counter, Dlet e)) ∧ (
+    compile_dec counter dec = (counter, dec))`
 
-val compile_dec_def = Define`
-  compile_dec counter dec =
-    case dec of
-    | Dlet e =>
-      let (counter, e) = compile_exp counter [] e in
-      (counter, Dlet e)
-    | _ => (counter, dec)
-`
+val compile_decs_aux_def = Define
 
-val compile_decs_aux_def = Define`
-  compile_decs_aux counter decs =
-    case decs of
-    | [] => counter, []
-    | dec::decs =>
+  `(compile_decs_aux counter [] = (counter, [])) ∧ (
+    compile_decs_aux counter (dec::decs) =
       let (counter, dec) = compile_dec counter dec in
       let (counter, decs) = compile_decs_aux counter decs in
-      counter, dec::decs
-`
+      counter, dec::decs)`
 
-val compile_decs_def = Define`
-  compile_decs decs =
-    SND (compile_decs_aux 0 decs)
-`
+val compile_decs_def = Define
 
+  `compile_decs decs = SND (compile_decs_aux 0 decs)`
 
 val _ = export_theory ()
