compiler/backend/proofs/flat_scopeAnalysisProofScript.sml
@@ -5,8 +5,13 @@ open
   flatLangTheory
   flatSemTheory
   flat_scopeAnalysisTheory
+  flat_parameterLiftingSolveTheory
   semanticsTheory
   basicSizeTheory
+  set_utilsTheory
+  mlnumTheory
+  mlstringTheory
+  ASCIInumbersTheory
 
 val _ = new_theory "flat_scopeAnalysisProof"
 
@@ -59,7 +64,7 @@ val alpha_eq_p_trans = Q.store_thm("alpha_eq_p_trans",
 >- (Cases_on `ps''` >> fs[alpha_eq_p_def]))
 
 (* TODO: dddddddddd *)
-fun progress tac = (fn g => let val (g',v) = tac g in if [g] = g' then failwith "foo" else (g', v) end)
+(* fun progress tac = (fn g => let val (g',v) = tac g in if [g] = g' then failwith "foo" else (g', v) end)*)
 
 val extract_repl_p_def = tDefine "extract_repl_p" `
 
@@ -67,19 +72,44 @@ val extract_repl_p_def = tDefine "extract_repl_p" `
   (extract_repl_p (Pcon _ l) (Pcon _ l') = extract_repl_ps l l') ∧
   (extract_repl_p (Pref p) (Pref p') = extract_repl_p p p') ∧
   (extract_repl_p _ _ = []) ∧
-  (extract_repl_ps [] _ = []) ∧
-  (extract_repl_ps _ [] = []) ∧
-  (extract_repl_ps (h::t) (h'::t') = (extract_repl_p h h') ++ (extract_repl_ps t t'))`
+  (extract_repl_ps (h::t) (h'::t') = (extract_repl_p h h') ++ (extract_repl_ps t t')) ∧
+  (extract_repl_ps _ _ = [])`
 
   (WF_REL_TAC `inv_image $< (λ x. case x of
     | INL (p, _) => pat_size p
     | INR (ps, _) => pat1_size ps
   )`)
 
+(* TODO: useless :) *)
+val extract_repl_exp_def = tDefine "extract_repl_exp"
+  `(extract_repl_exp (Raise _ e) (Raise _ e') = extract_repl_exp e e') ∧
+   (extract_repl_exp (Handle _ e pes) (Handle _ e' pes') = (extract_repl_exp e e') ++ (extract_repl_pes pes pes')) ∧
+   (extract_repl_exp (Lit _ _) (Lit _ _) = []) ∧
+   (extract_repl_exp (Con _ _ es) (Con _ _ es') = extract_repl_es es es') ∧
+   (extract_repl_exp (Var_local _ _) (Var_local _ _) = []) ∧
+   (extract_repl_exp (Fun _ x e) (Fun _ x' e') = (x, x')::(extract_repl_exp e e')) ∧
+   (extract_repl_exp (App _ _ es) (App _ _ es') = extract_repl_es es es') ∧
+   (extract_repl_exp (If _ e1 e2 e3) (If _ e1' e2' e3') =
+      (extract_repl_exp e1 e1') ++ (extract_repl_exp e2 e2') ++ (extract_repl_exp e3 e3')) ∧
+   (extract_repl_exp (Mat _ e pes) (Mat _ e' pes') = (extract_repl_exp e e') ++ (extract_repl_pes pes pes')) ∧
+   (extract_repl_exp (Let _ x e1 e2) (Let _ x' e1' e2') =
+      (case x, x' of | SOME x, SOME x' => [(x, x')] | _, _ => []) ++
+      (extract_repl_exp e1 e1') ++ (extract_repl_exp e2 e2')) ∧
+   (extract_repl_exp (Letrec _ funs e) (Letrec _ funs' e') =
+      (extract_repl_funs funs funs') ++ (extract_repl_exp e e')) ∧
+   (extract_repl_funs ((fName, vName, e)::t) ((fName', vName', e')::t') =
+      (fName, fName')::(vName, vName')::(extract_repl_exp e e') ++ (extract_repl_funs t t')) ∧
+   (extract_repl_funs _ _ = []) ∧
+   (extract_repl_es (h::t) (h'::t') = (extract_repl_exp h h') ++ (extract_repl_es t t')) ∧
+   (extract_repl_es _ _ = []) ∧
+   (extract_repl_pe (p, e) (p', e') = (extract_repl_p p p') ++ (extract_repl_exp e e')) ∧
+   (extract_repl_pes (h::t) (h'::t') = (extract_repl_pe h h') ++ (extract_repl_pes t t')) ∧
+   (extract_repl_pes _ _ = [])`
+
 val alpha_eq_exp_def = tDefine "alpha_eq_exp" `
-  (alpha_eq_pe repl (p, e) (p', e') = (alpha_eq_p p p' ∧ alpha_eq_exp ((extract_repl_p p p') ++ repl) e e')) ∧
-  (alpha_eq_pes _ [] [] =T) ∧
-  (alpha_eq_pes repl (h::t) (h'::t') = (alpha_eq_pe repl h h' ∧ alpha_eq_pes repl t t')) ∧
+  (alpha_eq_pe repl p e p' e' = (alpha_eq_p p p' ∧ alpha_eq_exp ((extract_repl_p p p') ++ repl) e e')) ∧
+  (alpha_eq_pes _ [] [] = T) ∧
+  (alpha_eq_pes repl ((p, e)::t) ((p',e')::t') = (alpha_eq_pe repl p e p' e' ∧ alpha_eq_pes repl t t')) ∧
   (alpha_eq_pes _ _ _  = F) ∧
   (alpha_eq_es _ [] [] = T) ∧
   (alpha_eq_es repl (e::t) (e'::t') = (alpha_eq_exp repl e e' ∧ alpha_eq_es repl t t')) ∧
@@ -115,7 +145,7 @@ val alpha_eq_exp_def = tDefine "alpha_eq_exp" `
   (alpha_eq_funs _ _ _ = F)`
 
   (WF_REL_TAC `inv_image $< (λ x. case x of
-    | INL (_, pe, _) => exp5_size pe
+    | INL (_, p, e, _, _) => exp5_size (p, e)
     | INR (INL (_, pes, _)) => exp3_size pes
     | INR (INR (INL (_, es, _))) => exp6_size es
     | INR (INR (INR (INL (_, e, _)))) => exp_size e
@@ -170,7 +200,7 @@ val alpha_eq_exp_ind = theorem "alpha_eq_exp_ind"
 
 val alpha_eq_exp_refl = Q.store_thm("alpha_eq_exp_refl",
 
- `(∀ l pe pe'. (pe = pe' ∧ repl_valid_refl l) ⇒ alpha_eq_pe l pe pe') ∧
+ `(∀ l p e p' e'. (p = p' ∧ e = e' ∧ repl_valid_refl l) ⇒ alpha_eq_pe l p e p' e') ∧
   (∀ l pes pes'. (pes = pes'∧ repl_valid_refl l) ⇒  alpha_eq_pes l pes pes') ∧
   (∀ l es es'. (es = es' ∧ repl_valid_refl l) ⇒ alpha_eq_es l es es') ∧
   (∀ l exp exp'. (exp = exp' ∧ repl_valid_refl l) ⇒ alpha_eq_exp l exp exp') ∧
@@ -209,17 +239,6 @@ val alpha_eq_exp_refl = Q.store_thm("alpha_eq_exp_refl",
 val repl_valid_sym_def = Define
 
   `repl_valid_sym (l : (tvarN, tvarN) alist) =
-   ∀ x y. case ALOOKUP l x of
-   | NONE => (case ALOOKUP (MAP SWAP l) y of
-     | NONE => T
-     | SOME x' => x ≠ x')
-   | SOME y' => (case ALOOKUP (MAP SWAP l) y' of
-     | NONE => F
-     | SOME x' => x' = x)`
-
-val repl_valid_sym_def = Define
-
-  `repl_valid_sym (l : (tvarN, tvarN) alist) =
    ∀ x y. (ALOOKUP           l  x = SOME y ⇒ ALOOKUP (MAP SWAP l) y = SOME x) ∧
           (ALOOKUP (MAP SWAP l) y = SOME x ⇒ ALOOKUP           l  x = SOME y)`
 
@@ -253,21 +272,15 @@ val ALOOKUP_MAP_SWAP2 = Q.store_thm("ALOOKUP_MAP_SWAP2",
 >> rw[]
 >> res_tac)
 
-val extract_valid_sym = Q.store_thm("extract_valid_sym",
-
-  `(∀ p p'. extract_repl_p p p' = MAP SWAP (extract_repl_p p' p)) ∧
-   (∀ ps ps'. extract_repl_ps ps ps' = MAP SWAP (extract_repl_ps ps' ps))`,
-
+val MAP_SWAP_extract_repl_p = Q.store_thm("MAP_SWAP_extract_repl_p",
+  `(∀ p p'. MAP SWAP (extract_repl_p p' p) = extract_repl_p p p' ) ∧
+   (∀ ps ps'. MAP SWAP (extract_repl_ps ps' ps) = extract_repl_ps ps ps')`,
    ho_match_mp_tac alpha_eq_p_ind
 >> rw[extract_repl_p_def, SWAP_def])
 
 val map_swap_swap_id = Q.store_thm("map_swap_swap_id",
-
   `∀ l. MAP SWAP (MAP SWAP l) = l`,
-
-   Induct_on `l`
->> simp[]
->> rw[SWAP_def])
+   Induct_on `l` >> simp[] >> rw[SWAP_def])
 
 val repl_valid_sym_sym = Q.store_thm("repl_valid_sym_sym",
 
@@ -275,8 +288,8 @@ val repl_valid_sym_sym = Q.store_thm("repl_valid_sym_sym",
 
    fs[repl_valid_sym_def, map_swap_swap_id, SWAP_def])
 
-(* TODO *)
-val extract_valid_sym = Q.store_thm("extract_valid_sym",
+(* TODO
+val extract_repl_p_repl_valid_sym = Q.store_thm("extract_repl_p_repl_valid_sym",
 
   `(∀ p p'. repl_valid_sym (extract_repl_p p p') ⇒ repl_valid_sym (extract_repl_p p' p)) ∧
    (∀ ps ps'. repl_valid_sym (extract_repl_ps ps ps') ⇒ repl_valid_sym (extract_repl_ps ps' ps))`,
@@ -293,16 +306,502 @@ val extract_valid_sym = Q.store_thm("extract_valid_sym",
 
 >- qmatch_rename_tac `repl_valid_sym (l1 ++ l2)`)
 
+val alpha_eq_repl_valid_sym = Q.store_thm("alpha_eq_repl_valid_sym"
+ `(∀ p p'. alpha_eq_p p p' ⇒ repl_valid_sym (extract_repl_p p p')) ∧
+  (∀ ps ps'. alpha_eq_ps ps ps' ⇒ repl_valid_sym (extract_repl_ps ps ps'))`,
+
+  ho_match_mp_tac alpha_eq_p_ind >>
+  rw[repl_valid_sym_def, extract_repl_p_def, alpha_eq_p_def, SWAP_def] >>
+  fs[ALOOKUP_APPEND] >>
+
+  CASE_TAC >> fs[] >>
+    >-(FULL_CASE_TAC
+       >- fs[ALOOKUP_MAP_SWAP]
+       >- (fs[] >> imp_res_tac ALOOKUP_MAP_SWAP))
+    >-(FULL_CASE_TAC
+       >- fs[ALOOKUP_MAP_SWAP]
+       >- (fs[] >> imp_res_tac ALOOKUP_MAP_SWAP)
+       )
+
+
+
+
+  EVERY_CASE_TAC >> res_tac >> rw[] >> fs[] >>
+
+
+     fs[ALOOKUP_MAP_SWAP2]
+     rw[]
+  )
+  >-
+  fs[ALOOKUP_]
+
+  res_tac
+  res_tac >>
+  [MAP_APPEND,]
+  Cases_on`p'` >>
+  fs[extract_repl_p_def,SWAP_def]
+  ALOOKUP_MAP_SWAP
+  find"alpha_eq_p"
+  >-
+  >-
+  >-
+  >-
+  MAP_SWAP_extract_repl_p,] >>
+
 val alpha_eq_exp_sym = Q.store_thm("alpha_eq_exp_sym",
 
-  `(∀ l pe pe'. (repl_valid_sym l ∧ alpha_eq_pe l pe pe') ⇒ alpha_eq_pe l pe' pe) ∧
-   (∀ l pes pes'. (repl_valid_sym l ∧ (alpha_eq_pes l pes pes' ⇒ alpha_eq_pes l pes' pes)) ∧
-   (∀ l es es'. (repl_valid_sym l ∧ alpha_eq_es l es es') ⇒ alpha_eq_es l es' es) ∧
-   (∀ l exp exp'. (repl_valid_sym l ∧ alpha_eq_exp l exp exp') ⇒ alpha_eq_exp l exp' exp) ∧
-   (∀ l f f'. (repl_valid_sym l ∧ alpha_eq_fun l f f') ⇒ alpha_eq_fun l f' f) ∧
-   (∀ l funs funs'. (repl_valid_sym ∧ alpha_eq_funs l funs funs') ⇒ alpha_eq_funs l funs' funs)`,
+  `(∀ l p e p' e'. (repl_valid_sym l ∧ alpha_eq_pe l p e p' e') ⇒ alpha_eq_pe (MAP SWAP l) p' e' p e) ∧
+   (∀ l pes pes'. (repl_valid_sym l ∧ alpha_eq_pes l pes pes') ⇒ alpha_eq_pes (MAP SWAP l) pes' pes) ∧
+   (∀ l es es'. (repl_valid_sym l ∧ alpha_eq_es l es es') ⇒ alpha_eq_es (MAP SWAP l) es' es) ∧
+   (∀ l exp exp'. (repl_valid_sym l ∧ alpha_eq_exp l exp exp') ⇒ alpha_eq_exp (MAP SWAP l) exp' exp) ∧
+   (∀ l f f'. (repl_valid_sym l ∧ alpha_eq_fun l f f') ⇒ alpha_eq_fun (MAP SWAP l) f' f) ∧
+   (∀ l funs funs'. (repl_valid_sym l ∧ alpha_eq_funs l funs funs') ⇒ alpha_eq_funs (MAP SWAP l) funs' funs)`,
+
+   ho_match_mp_tac alpha_eq_exp_ind >>
+   rw[alpha_eq_exp_def] >>
+   fs[alpha_eq_exp_def,alpha_eq_p_sym, extract_repl_p_valid_sym] >>
+   >-
+   >-
+   >-
+   >-
+   >-
+   >-
+   >-
+   )
+
+*)
+
+val is_closed_term_exp_def = Define
+
+  `is_closed_term_exp e = (compute_freeID_exp [] e = empty_set)`
+
+val _ = temp_overload_on("alist_dom", ``λ l. MAP FST l``)
+
+val _ = temp_overload_on("is_valid_term_exp",  ``λ l e. compute_freeID_exp  (alist_dom l) e = empty_set``)
+val _ = temp_overload_on("is_valid_term_pe",   ``λ l e. compute_freeID_pe   (alist_dom l) e = empty_set``)
+val _ = temp_overload_on("is_valid_term_pes",  ``λ l e. compute_freeID_pes  (alist_dom l) e = empty_set``)
+val _ = temp_overload_on("is_valid_term_fun",  ``λ l e. compute_freeID_fun  (alist_dom l) e = empty_set``)
+val _ = temp_overload_on("is_valid_term_funs", ``λ l e. compute_freeID_funs (alist_dom l) e = empty_set``)
+val _ = temp_overload_on("is_valid_term_es",   ``λ l e. compute_freeID_exps (alist_dom l) e = empty_set``)
+
+val alist_injective_def = Define
+
+  `alist_injective l =
+     ∀ x y z. ( ALOOKUP l x = SOME z ∧ ALOOKUP l y = SOME z ) ⇒ (x = y)`
+
+val alist_rename_format_ok_def = Define
+
+  `alist_rename_format_ok l n = ∀ x y. MEM (x, y) l ⇒ ∃ k. k < n ∧ y = mk_unique_name k x`
+
+val alist_rename_ok_def = Define
+
+  `alist_rename_ok l n = (alist_injective l ∧ alist_rename_format_ok l n)`
+
+val num_toString_bij = Q.store_thm("num_toString_bij",
+
+  `∀ n n'. num_toString n = num_toString n' ⇔ n = n'`,
+
+  metis_tac[num_to_dec_string_def, num_toString_thm, toString_11])
+
+val toString_bij = Q.store_thm("toString_bij",
+
+  `∀ n n'. n = n' ⇔ toString n = toString n'`,
+
+   rw[toString_def, implode_def]
+>> metis_tac[num_toString_bij])
+
+val mk_unique_bij1 = Q.store_thm("mk_unique_bij1",
+
+  `∀ k k' s s'. (k = k' ∧ s = s') ⇒ mk_unique_name k s = mk_unique_name k' s'`,
+
+  rw[mk_unique_name_def, STRCAT])
+
+val mk_unique_bij2 = Q.store_thm("mk_unique_bij2",
+
+  `∀ k k' s s'. mk_unique_name k s = mk_unique_name k' s' ⇒ (k = k' ∧ s = s')`,
+
+  cheat (* this is true because "_" can't be in a number, proof will not be trivial...*))
+
+val mk_unique_bij = Q.store_thm("mk_unique_big",
+
+  `∀ k k' s s'. mk_unique_name k s = mk_unique_name k' s' ⇔ (k = k' ∧ s = s')`,
+
+  metis_tac[mk_unique_bij1, mk_unique_bij2])
+
+val compile_funs_le = Q.store_thm("compile_funs_le",
+
+ `∀ funs n l. n ≤ FST (compile_name_rec_funs n l funs)`,
+
+  cheat
+  (* TODO: this doesn't work anymore
+   Induct >> rw[] >> fs[compile_name_rec_funs_def]
+>> rpt (pairarg_tac >> fs[])
+>> Cases_on`h` >> Cases_on`r`
+>> fs[compile_name_rec_fun_def]
+>> rw[]
+>> qmatch_asmsub_abbrev_tac `compile_name_rec_funs n0 l0`
+>> first_x_assum (assume_tac o Q.SPECL [`n0`,`l0`])
+>> unabbrev_all_tac
+>> rfs[]*))
+
+val compile_p_le = Q.store_thm("compile_p_le",
+
+  `(∀ p n l. n ≤ FST (compile_p n l p)) ∧
+   (∀ ps n l. n ≤ FST (compile_ps n l ps))`,
+
+   Induct
+>> fs[compile_p_def]
+>> rpt (pairarg_tac >> fs[])
+>> Induct
+>> rw[]
+>> rpt (pairarg_tac >> fs[])
+>> metis_tac[FST, LESS_EQ_TRANS])
+
+val compile_count_le = Q.store_thm("compile_count_le",
+
+  `(∀ n l el n' el'. compile_exp n l el  = (n', el') ⇒ n ≤ n') ∧
+   (∀ n l el n' el'. compile_fun n l el  = (n', el') ⇒ n ≤ n') ∧
+   (∀ n l el n' el'. compile_funs n l el = (n', el') ⇒ n ≤ n') ∧
+   (∀ n l el n' el'. compile_exps n l el = (n', el') ⇒ n ≤ n') ∧
+   (∀ n l el n' el'. compile_pe n l el   = (n', el') ⇒ n ≤ n') ∧
+   (∀ n l el n' el'. compile_pes n l el  = (n', el') ⇒ n ≤ n')`,
+
+   ho_match_mp_tac compile_exp_ind
+>> rw[compile_exp_def, compile_name_rec_funs_def, compile_funs_le]
+>> rpt(pairarg_tac >> fs[])
+>> rw[]
+>> metis_tac[compile_funs_le, compile_p_le, FST, LESS_EQ_TRANS])
+
+val ALIST_MAP_FST_SWAP_MAP_SND = Q.store_thm("ALIST_MAP_FST_SWAP_MAP_SND",
+
+  `∀ l. MAP FST (MAP SWAP l) = MAP SND l`,
+
+   Induct
+>> rw[SWAP_def, FST])
+
+val ALOOKUP_MEM_ADD = Q.store_thm("ALOOKUP_MEM_ADD",
+
+  `∀ l h x y. ALOOKUP (h::l) x = SOME y ⇒ (y = SND h ∨ MEM y (MAP SND l))`,
+
+   Induct
+>> Cases_on `h`
+>> rw[]
+>- metis_tac[])
+
+val ALOOKUP_SOME_MAP_SND = Q.store_thm("ALOOKUP_SOME_MAP_SND",
+
+  `∀ l x y. (ALOOKUP l x = SOME y) ⇒ MEM y (MAP SND l)`,
+
+   Induct
+>> rw[]
+>> rw[ALOOKUP_def, ALOOKUP_MEM, SND]
+>> metis_tac[ALOOKUP_MEM_ADD])
+
+val MEM_SWAP = Q.store_thm("MEM_SWAP",
+
+  `∀ l x y. MEM (x, y) l ⇔ MEM (y, x) (MAP SWAP l)`,
+
+  Induct
+>- rw[]
+>- ( rw[]
+  >> `(x, y) = h ⇒ (y, x) = SWAP h` by metis_tac[SWAP_def, FST, SND]
+  >> `(y, x) = SWAP h ⇒ (x, y) = h` by (EVAL_TAC >> fs[])
+  >> metis_tac[]))
+
+(*
+val ALOOKUP_SWAP_NONE_SOME = Q.store_thm("ALOOKUP_SWAP_NONE_SOME",
+
+  `∀ l x x'. ALOOKUP l x = SOME x' ⇔ ALOOKUP (MAP SWAP l) x' ≠ NONE`,
+
+   Induct
+>- rw[]
+>> rw[]
+>> Cases_on `h`
+>> rw[SWAP_def, ALOOKUP_MEM, ALOOKUP_def, ALOOKUP_MAP_SWAP, ALOOKUP_MAP_SWAP2])
+*)
+
+val compute_freeID_still_empty_included = Q.store_thm("compute_freeID_still_empty_included",
+
+  `∀ e e1 e2. (set_included e1 e2 ∧ compute_freeID_exp e1 e = empty_set) ⇒ compute_freeID_exp e2 e = empty_set`,
+
+  cheat)
+
+val compile_name_rec_funs_ok = Q.store_thm("compile_name_rec_funs_ok",
+
+  `∀ n l funs n' l' funs' n'' funs''.
+      compile_name_rec_funs n l funs = (n', l', funs') ∧
+      compile_funs n' l' funs' = (n'', funs'')
+      ⇒ l' = MAP2 (λ x y. FST x, FST y) funs funs'' ++ l`,
+
+  cheat
+(*
+   Induct_on `funs`
+>> fs[compile_name_rec_funs_def, compile_exp_def]
+>> rw[]
+>> Cases_on `funs'`
+>> rw[]
+>> fs[compile_name_rec_funs_def, compile_exp_def]
+>> rw[]
+>> rpt (pairarg_tac >> fs[])
+>> rw[]
+>> Cases_on `f`
+>> fs[compile_exp_def]
+>> rpt(pairarg_tac >> fs[])
+>> rw[]
+>> Cases_on `h`
+>> fs[]
+>> Cases_on`r'`
+>> fs[compile_name_rec_funs_def, compile_name_rec_fun_def]
+(* TODO: move compile_name_rec_fun directly into compile_name_rec_funs *)
+>> rw[]
+
+>> Cases_on`l'`
+>- (
+     fs[compile_exp_def]
+     pairarg_tac >> fs[]
+     rw[]
+     cheat)
+>> rw[compile_exp_def]
+>> rw[compile_name_rec_fun_def]
+
+res_tac
+
+>> cheat
+*))
+
+val compute_freeID_still_empty_less_funs = Q.store_thm("compute_freeID_still_empty_less_funs",
+
+  `∀ l f funs. compute_freeID_funs l (f::funs) = empty_set ⇒ compute_freeID_funs l funs = empty_set`,
+
+  cheat)
+
+
+val is_valid_less_funs = Q.store_thm("is_valid_less_funs",
+
+  `∀ l f funs. is_valid_term_funs l (f::funs) ⇒ is_valid_term_funs l funs`,
+
+   metis_tac[compute_freeID_still_empty_less_funs])
+
+val is_valid_term_funs_fun = Q.store_thm("is_valid_term_funs_fun",
+
+  `∀ l fName q r funs. is_valid_term_funs l ((fName, q, r):: funs) ⇒ is_valid_term_fun l (q, r)`,
 
    cheat)
+
+val rename_p_alpha_eq = Q.store_thm("rename_p_alpha_eq",
+
+  `(∀ n l p p' l' n'.
+    compile_p n l p = (n', l', p') ⇒ alpha_eq_p p p') ∧
+   (∀ n l p p' l' n'.
+    compile_ps n l p = (n', l', p') ⇒ alpha_eq_ps ps ps')`,
+
+   cheat)
+
+val rename_alpha_eq = Q.store_thm("rename_alpha_eq",
+
+  `(∀ n l e e' n'.
+      ((is_valid_term_exp l e) ∧
+       ((n', e') = compile_exp n l e) ∧
+       (alist_rename_ok l n))
+      ⇒ alpha_eq_exp l e e') ∧
+   (∀ n l f f' n'.
+      ((is_valid_term_fun l f) ∧
+       ((n', f') = compile_fun n l f) ∧
+       (alist_rename_ok l n))
+      ⇒ alpha_eq_fun l f f') ∧
+   (∀ n l funs funs' n'.
+      ((is_valid_term_funs l funs) ∧
+       ((n', funs') = compile_funs n l funs) ∧
+       (alist_rename_ok l n))
+      ⇒ alpha_eq_funs l funs funs') ∧
+   (∀ n l es es' n'.
+      ((is_valid_term_es l es) ∧
+       ((n', es') = compile_exps n l es) ∧
+       (alist_rename_ok l n))
+      ⇒ alpha_eq_es l es es') ∧
+  (∀ n l pe pe' n'.
+       ((is_valid_term_pe l pe) ∧
+        ((n', pe') = compile_pe n l pe) ∧
+        (alist_rename_ok l n))
+       ⇒ alpha_eq_pe l (FST pe) (SND pe) (FST pe') (SND pe')) ∧
+   (∀ n l pes pes' n'.
+      ((is_valid_term_pes l pes) ∧
+       ((n', pes') = compile_pes n l pes) ∧
+       (alist_rename_ok l n))
+      ⇒ alpha_eq_pes l pes pes')`,
+
+   ho_match_mp_tac compile_exp_ind
+>> rw[alpha_eq_exp_def, compile_exp_def, alist_rename_ok_def, alist_rename_format_ok_def, alist_injective_def]
+>> rpt(pairarg_tac >> fs[])
+>> rw[alpha_eq_exp_def]
+>> fs[compute_freeID_exp_def]
+>> res_tac
+>- ( first_x_assum match_mp_tac
+  >> imp_res_tac set_union_empty)
+>- ( first_x_assum match_mp_tac
+   >> rw[compile_exp_def]
+   >> `n ≤ counter'` by metis_tac [FST, LESS_EQ_TRANS, compile_p_le, compile_count_le]
+  >> rw[]
+  >- imp_res_tac set_union_empty
+  >> res_tac
+  >> qexists_tac `k`
+  >> rw[])
+>- ( CASE_TAC >- ( imp_res_tac ALOOKUP_NONE >> fs[set_add_non_empty])
+  >> CASE_TAC >- imp_res_tac ALOOKUP_MAP_SWAP >>
+    imp_res_tac ALOOKUP_MEM >>
+    imp_res_tac MEM_SWAP >>
+    res_tac >> metis_tac[mk_unique_bij])
+>- ( first_x_assum match_mp_tac
+  >> rw[]
+  >- ( `set_included (set_add (alist_dom l) x) (x::(alist_dom l))` by (rw[set_included_def] >> metis_tac[set_add_thm])
+    >> metis_tac[compute_freeID_still_empty_included])
+  >- ( rw[]
+    >> imp_res_tac ALOOKUP_MEM
+    >> res_tac
+    >> metis_tac[mk_unique_bij])
+  >- ( rw[]
+    >> imp_res_tac ALOOKUP_MEM
+    >> res_tac
+    >> metis_tac[mk_unique_bij])
+  >- ( qexists_tac `n` >> rw[])
+  >- ( res_tac >> qexists_tac `k` >> rw[]))
+>- ( first_x_assum match_mp_tac >> imp_res_tac set_union_empty)
+>- ( first_x_assum match_mp_tac
+  >> NTAC 2 (imp_res_tac set_union_empty)
+  >> fs[]
+  >> rw[]
+  >> res_tac
+  >> qexists_tac `k`
+  >> rw[]
+  >> `n ≤ counter'` by metis_tac[compile_count_le]
+  >> fs[LESS_EQ_LESS_TRANS, LESS_EQ_TRANS])
+>- ( first_x_assum match_mp_tac
+  >> NTAC 2 (imp_res_tac set_union_empty)
+  >> fs[]
+  >> rw[]
+  >> res_tac
+  >> qexists_tac `k`
+  >> rw[]
+  >> `n ≤ counter''` by metis_tac[compile_count_le, LESS_EQ_TRANS]
+  >> fs[LESS_EQ_TRANS, LESS_EQ_LESS_TRANS])
+>- ( first_x_assum match_mp_tac >> imp_res_tac set_union_empty)
+>- ( first_x_assum match_mp_tac
+  >> imp_res_tac set_union_empty
+  >> fs[]
+  >> rw[]
+  >> res_tac
+  >> qexists_tac `k`
+  >> fs[]
+  >> `n ≤ counter'` by metis_tac[compile_count_le, LESS_EQ_TRANS]
+  >> res_tac
+  >> fs[LESS_EQ_TRANS, LESS_EQ_LESS_TRANS])
+>- ( first_x_assum match_mp_tac
+  >> imp_res_tac set_union_empty
+  >> fs[]
+  >> rw[]
+  >> fs[]
+  >> res_tac
+  >> qexists_tac `k`
+  >> fs[])
+>- ( first_x_assum match_mp_tac
+  >> rw[]
+  >- ( imp_res_tac set_union_empty
+    >> `set_included (set_union (alist_dom l) [x]) (x::alist_dom l)` by metis_tac[set_eq_union_sing_app, set_eq_imp_incl]
+    >> metis_tac[compute_freeID_still_empty_included])
+  >- metis_tac[mk_unique_bij,ALOOKUP_MEM]
+  >- metis_tac[mk_unique_bij,ALOOKUP_MEM]
+  >- ( qexists_tac `n`
+    >> rw[]
+    >> `n + 1 ≤ counter'` by metis_tac[compile_count_le, LESS_EQ_TRANS]
+    >> fs[])
+  >- ( res_tac
+    >> qexists_tac `k`
+    >> `n + 1 ≤ counter'` by metis_tac[compile_count_le, LESS_EQ_TRANS]
+    >> fs[]))
+>- ( first_x_assum match_mp_tac >> imp_res_tac set_union_empty)
+>- ( first_x_assum match_mp_tac
+  >> imp_res_tac compile_count_le
+  >> rw[]
+  >- ( imp_res_tac set_union_empty
+    >> `set_included (set_union (alist_dom l) empty_set) (alist_dom l)` by metis_tac[set_union_empty_id, set_eq_imp_incl]
+    >> metis_tac[compute_freeID_still_empty_included])
+  >- ( res_tac
+    >> qexists_tac `k `
+    >> rw[]))
+>- ( imp_res_tac set_union_empty
+  >> imp_res_tac compile_name_rec_funs_ok
+  >> sg `is_valid_term_exp repl' e`
+    >- ( imp_res_tac compile_name_rec_funs_ok
+      >> fs[]
+      >> rw[]
+      (*>> sg `(alist_dom (MAP2 (λ x y. (FST x, FST y)) funs funs'')) = (MAP (λ (name, _, _). name) funs)`
+        >- cheat*)
+      >> cheat)
+  >> fs[]
+  >> rfs[]
+  >> rw[]
+  >> cheat)
+>- ( imp_res_tac set_union_empty
+  >> imp_res_tac compile_name_rec_funs_ok
+  >> cheat)
+>- ( first_x_assum match_mp_tac
+  >> rw[]
+  >> `set_eq (vName::alist_dom l) (set_add (alist_dom l) vName)` by (
+          rw[set_eq_def]
+        >> EQ_TAC
+        >> rw[MEM, set_add_def]
+        >> metis_tac[set_add_thm])
+  >- metis_tac[compute_freeID_still_empty_included, set_eq_imp_incl]
+  >- ( `MEM (y, mk_unique_name n vName) l` by metis_tac[ALOOKUP_MEM]
+    >> res_tac
+    >> metis_tac[mk_unique_bij])
+  >- ( `MEM (x, mk_unique_name n vName) l` by metis_tac[ALOOKUP_MEM]
+    >> res_tac
+    >> metis_tac[mk_unique_bij])
+  >- ( qexists_tac `n`
+    >> rw[])
+  >- ( res_tac
+    >> qexists_tac `k`
+    >> rw[]))
+>- ( Cases_on `f`
+  >> Cases_on` f'`
+  >> fs[alpha_eq_exp_def]
+  >> rw[]
+  >> imp_res_tac is_valid_less_funs
+  >> `n ≤ counter'` by metis_tac[compile_count_le]
+  >- metis_tac[is_valid_term_funs_fun]
+  >> first_x_assum match_mp_tac
+  >> rw[]
+  >> res_tac
+  >> qexists_tac`k`
+  >> fs[]
+  >> imp_res_tac compile_count_le
+  >> fs[])
+>- ( first_x_assum match_mp_tac >> imp_res_tac set_union_empty)
+>- ( first_x_assum match_mp_tac
+  >> imp_res_tac set_union_empty
+  >> rw[]
+  >> res_tac
+  >> qexists_tac `k`
+  >> `n ≤ counter'` by metis_tac[compile_count_le, LESS_EQ_TRANS]
+  >> fs[])
+>- metis_tac[rename_p_alpha_eq]
+>- ( `n ≤ counter'` by metis_tac[compile_p_le, LESS_EQ_LESS_TRANS, LESS_EQ_LESS_TRANS, FST]
+  >> `set_eq (extract_repl_p p p' ++ l) repl'` by cheat
+  (* TODO: rewrite compile_p_def so we only return new repl, not the old one updated ; should make this easier... *)
+  >> cheat)
+>- ( imp_res_tac set_union_empty
+  >> rw[])
+>- ( imp_res_tac set_union_empty
+  >> rw[])
+>- ( first_x_assum match_mp_tac
+  >> imp_res_tac set_union_empty
+  >> rw[]
+  >> res_tac
+  >> qexists_tac `k`
+  >> `n ≤ counter''` by metis_tac[compile_p_le, LESS_EQ_TRANS, LESS_EQ_LESS_TRANS, FST]
+  >> `counter'' ≤ counter'` by metis_tac[compile_count_le, LESS_EQ_TRANS]
+  >> fs[]))
 
 val alpha_eq_dec_def = Define
 
@@ -313,18 +812,29 @@ val alpha_eq_dec_def = Define
 
 val alpha_eq_dec_ind = theorem "alpha_eq_dec_ind"
 
-val rename_dec_alpha_eq = Define
+val is_valid_dec_def = Define `
+  (is_valid_dec (Dlet e) = (compute_freeID_exp [] e = empty_set)) ∧
+  (is_valid_dec (Dtype _ _) = T) ∧
+  (is_valid_dec (Dexn _ _) = T)
+`
 
-  `∀ dec n. (n', dec') = flat_scopeAnalysis$compile_dec n dec ⇒ alpha_eq_dec dec dec'`
+val rename_dec_alpha_eq = Q.store_thm("rename_dec_alpha_eq",
+
+  `∀ dec n. (is_valid_dec dec ∧ (n', dec') = compile_dec n dec) ⇒ alpha_eq_dec dec dec'`,
 
    rw[]
->> Induct_on `dec`
->> Induct_on `e`
->> Induct_on `dec'`
->> simp[compile_dec_def]
->> rw[]
->> rw[compile_exp_def]
->> cheat
+>> Cases_on `dec`
+>> Cases_on `dec'`
+>> rw[alpha_eq_dec_def, compile_dec_def]
+>> fs[alpha_eq_dec_def, compile_dec_def]
+>- ( fs[is_valid_dec_def]
+  >> `compile_exp n [] e = (n', e')` by (pairarg_tac >> fs[])
+  >> `is_valid_term_exp [] e` by (`alist_dom [] = []` by EVAL_TAC >> rw[])
+  >> `alist_rename_ok [] n` by rw[alist_rename_ok_def, alist_injective_def, alist_rename_format_ok_def]
+  >> imp_res_tac rename_alpha_eq
+  >> rw[])
+>> pairarg_tac
+>> fs[])
 
 val alpha_eq_decs_def = Define
 
@@ -332,37 +842,20 @@ val alpha_eq_decs_def = Define
    (alpha_eq_decs (h::t) (h'::t') = (alpha_eq_dec h h' ∧ alpha_eq_decs t t')) ∧
    (alpha_eq_decs _ _ = F)`
 
+val is_valid_decs_def = Define
+
+  `is_valid_decs decs = (∀ dec. MEM dec decs ⇒ is_valid_dec dec)`
+
 val rename_decs_alpha_eq = Q.store_thm("rename_decs_alpha_eq",
 
-  `∀ decs. decs' = flat_scopeAnalysis$compile_decs decs ⇒ alpha_eq_decs decs decs'`
+  `∀ decs. (is_valid_decs decs ∧ decs' = compile_decs decs) ⇒ alpha_eq_decs decs decs'`,
 
-   rw[]
+  Induct
+>- rw[alpha_eq_decs_def, rename_dec_alpha_eq, compile_decs_def, SND, compile_decs_aux_def]
+>> rw[]
 >> cheat)
 
-(* TODO *)
-val compile_exp_alpha_eq = Q.store_thm("compile_exp_alpha_eq",
-
-  `∀ exp exp'. (_, exp') = flat_scopeAnalysis$compile_exp 0 [] exp ⇒ alpha_eq_exp [] exp exp'`,
-
-)
-
 val alpha_eq_dec_ind = theorem "alpha_eq_dec_ind"
-
-(* TODO *)
-val compile_dec_alpha_eq = Q.store_thm("compile_dec_alpha_eq",
-
-  `∀ dec dec'. (_, dec') = flat_scopeAnalysis$compile_dec 0 dec ⇒ alpha_eq_dec dec dec'`,
-
-   ho_match_mp_tac alpha_eq_dec_ind
->> rw[]
->> fs[compile_decs_def]
->> ho_match_mp_tac alpha_eq_exp_ind)
-
-val compile_decs_alpha_eq = Q.store_thm("compile_decs_alpha_eq",
-
-  `∀ decs. decs' = flat_scopeAnalysis$compile_decs decs ⇒ alpha_eq_decs decs decs'`,
-
-   cheat)
 
 (* TODO *)
 
@@ -370,7 +863,7 @@ val compile_decs_alpha_eq = Q.store_thm("compile_decs_alpha_eq",
 val (t_rel_rules, t_rel_ind, t_rel_cases) = Hol_reln
 
    (* TODO: on each case, do we need to check anything on t ? *)
-  `(∀ env env' t t' e e'. t_rel env env' e e' ⇒ t_rel env env' (Raise t e) (Raise t e')) ∧
+  `(∀ env env' t t' e e'. t_rel env env' e e' ⇒ t_rel env env' (Raise t e) (Raise t' e')) ∧
    (∀ env env' t t' e e' pes pes'. (* TODO: do we need to check something about pes and pes' ? *) t_rel env env' e e' ⇒ t_rel env env' (Handle t e pes) (Handle t' e' pes')) ∧
    (∀ env env' t t' l l'. l = l' ⇒ t_rel env env' (Lit t l) (Lit t' l')) ∧
    (∀ env env' t t' id id' es es'. (* TODO: do we care about id ? *) LIST_REL t_rel es es' ⇒ t_rel env env' (Con t id es) (Con t' id' es')) ∧
