compiler/backend/set_utilsScript.sml
@@ -1,4 +1,4 @@
-open  preamble mlintTheory
+open preamble mlintTheory
 
 val _ = new_theory "set_utils"
 
@@ -8,10 +8,30 @@ val empty_set_def = Define
 
   `empty_set = []`
 
+val set_eq_def = Define
+
+  `set_eq e1 e2 = ∀ x. MEM x e1 ⇔ MEM x e2`
+
 val set_add_def = Define
 
-  `(set_add [] el =[el]) ∧
+  `(set_add [] el = [el]) ∧
    (set_add (h::t) el = h::(if h = el then t else set_add t el))`
+
+val set_add_thm = Q.store_thm("set_add_thm",
+
+  `∀ e el. MEM el (set_add e el)`,
+
+   Induct
+>> rw[set_add_def])
+
+val set_add_included = Q.store_thm("set_add_thm",
+
+  `∀ e1 el x. MEM x e1 ∨ x = el ⇔ MEM x (set_add e1 el)`,
+
+   Induct >> rw[set_add_def]
+>> EQ_TAC >> rw[]
+>> res_tac >> fs[]
+>> metis_tac[set_add_thm])
 
 val set_rm_def = Define
 
@@ -21,8 +41,17 @@ val set_rm_def = Define
 val set_union_def = Define
 
   `(set_union [] s = s) ∧
-   (set_union s [] = s) ∧
    (set_union (h::t) s = set_union t (set_add s h))`
+
+val set_union_thm = Q.store_thm("set_union_thm",
+
+  `∀ e1 e2 x. (MEM x e1 ∨ MEM x e2) ⇔ MEM x (set_union e1 e2)`,
+
+  Induct
+  >- ( Induct
+    >> rw[set_union_def, set_add_def])
+  >> rw[set_union_def, set_add_def]
+  >> metis_tac[set_add_thm, set_add_included])
 
 val set_big_union_def = Define
 
@@ -44,5 +73,106 @@ val set_img_def = Define
 
   `(set_img [] f = []) ∧
    (set_img (h::t) f = set_add (set_img t f) (f h))`
+
+val set_included_def = Define
+
+  `set_included e1 e2 = ∀ x. MEM x e1 ⇒ MEM x e2`
+
+val set_included_thm = Q.store_thm("set_included_thm",
+
+  `∀ el e1 e2. set_included e1 (el::e1) ∧ set_included e1 (set_add e1 el) ∧ set_included e1 (set_union e1 e2)`,
+
+  rw[set_included_def]
+  >- ( Induct_on `e1` >> NTAC 2 (rw[set_add_def]))
+  >- metis_tac[set_union_thm])
+
+val set_eq_imp_incl = Q.store_thm("set_eq_imp_incl",
+
+  `∀ e1 e2. set_eq e1 e2 ⇔ set_included e1 e2 ∧ set_included e2 e1`,
+
+   rw[set_eq_def, set_included_def]
+>> EQ_TAC
+>> metis_tac[set_eq_def])
+
+val set_eq_union_sing_app = Q.store_thm("set_eq_union_sing_app",
+
+  `∀ e1 el. set_eq (set_union e1 [el]) (el::e1)`,
+
+  Induct
+>- rw[set_eq_def, set_union_def]
+>- (
+  rw[set_eq_def, set_union_def]
+  >> EQ_TAC
+  >> `MEM el [el]` by fs[]
+  >> rw[]
+  >> (
+    fs[set_union_def, set_add_def]
+    >> EVERY_CASE_TAC
+    >> rw[]
+    >> metis_tac[set_union_thm, set_add_thm, MEM])))
+
+
+
+val set_add_non_empty = Q.store_thm("set_add_non_empty",
+
+  `∀ el e. set_add e el ≠ empty_set`,
+
+   Induct_on `e`
+>> rw[set_add_def, empty_set_def])
+
+val set_union_empty = Q.store_thm("set_union_empty",
+
+  `∀ e1 e2. (set_union e1 e2 = empty_set) ⇒ (e1 = empty_set ∧ e2 = empty_set)`,
+
+  `∀ e1 e2. (set_union e1 e2 = empty_set) ⇔ (e1 = empty_set ∧ e2 = empty_set)`
+  suffices_by fs[] >>
+   Induct_on `e1`
+>> fs[set_union_def, set_add_non_empty]
+>> rw[set_add_non_empty,empty_set_def])
+
+val set_union_empty_id = Q.store_thm("set_union_empty_id",
+
+  `∀ e1. set_eq (set_union e1 empty_set) e1`,
+
+  Induct
+  >> rw[set_eq_def, set_union_def, empty_set_def]
+  >> fs[set_add_def]
+  >> EQ_TAC >> rw[]
+  >- (imp_res_tac set_union_thm >> fs[])
+  >> `MEM h [h]` by fs[]
+  >> imp_res_tac set_union_thm >> fs[])
+
+val set_union_commut = Q.store_thm("set_union_commut",
+
+  `∀ e1 e2. set_eq (set_union e1 e2) (set_union e2 e1)`,
+
+  Induct
+  >-( Induct
+    >- rw[set_union_def, set_eq_def]
+    >- ( rw[]
+      >> fs[set_union_def,set_union_empty_id,empty_set_def, set_add_thm, set_add_def]
+      >> rw[set_eq_def]
+      >> `MEM h [h]` by fs[]
+      >> imp_res_tac set_union_thm
+      >> EQ_TAC
+      >> rw[]
+      >> fs[]
+      >- metis_tac[set_union_thm]
+      >> imp_res_tac set_union_thm
+      >> fs[]))
+  >-( Induct_on `e2`
+    >> rw[]
+    >- ( fs[set_union_def, set_eq_def,set_add_def]
+      >> rw[]
+      >> EQ_TAC
+      >> rw[]
+      >> fs[]
+      >> `MEM h [h]` by fs[]
+      >> imp_res_tac set_union_thm
+      >> fs[])
+    >- (
+      cheat
+      (* TODO *)
+    )))
 
 val _ = export_theory ()
